verif/verif_gotokey.v
@@ -1,4 +1,4 @@
-(** * verif_gotokey.v : Correctness proof of isNodeParent, AscendToParent and goToKey *)
+(** * verif_gotokey.v : Correctness proof of AscendToParent and goToKey *)
 
 Require Import VST.floyd.proofauto.
 Require Import VST.floyd.library.
@@ -16,46 +16,7 @@ Require Import index.
 Require Import btrees_sep.
 Require Import btrees_spec.
 Require Import verif_findindex.
-
-Lemma body_isNodeParent: semax_body Vprog Gprog f_isNodeParent isNodeParent_spec.
-Proof.
-  start_function.
-  forward_call(n,key).
-  forward_if(PROP() LOCAL(temp _t'2 (Val.of_bool (negb (isNodeParent n key))); temp _idx (rep_index (findChildIndex n key)); temp _node (getval n); temp _key (Vint (Int.repr key))) SEP (btnode_rep n)).
-  - forward.                    (* t'2=1 *)
-    entailer!.
-    destruct (findChildIndex n key) eqn:FCI.
-    unfold isNodeParent. rewrite FCI. simpl. auto.
-    inv H1. admit.              (* contradiction in h6 *)
-  - destruct n as [ptr0 le isLeaf First Last pn].
-    pose (n:=btnode val ptr0 le isLeaf First Last pn).
-    rewrite unfold_btnode_rep. simpl. Intros.
-    forward.                    (* t'3=node->numKeys *)
-    forward.                    (* t'2= (idx==t'3-1) *)
-    + admit.                    (* tc_expr *)
-    + gather_SEP 0 1 2 3. replace_SEP 0 (btnode_rep n).
-      { entailer!. }
-      entailer!.
-      unfold isNodeParent. fold n.
-      destruct (findChildIndex n key) eqn:FCI.
-      { unfold findChildIndex, n in FCI. rewrite FCI in H1. simpl in H1. inv H1. }
-      rewrite negb_involutive.
-      destruct (S n0 =? numKeys n)%nat eqn:Hnum.
-      * unfold findChildIndex, n in FCI. rewrite FCI.
-        simpl.
-        inv Hnum. destruct (numKeys_le le); inv H8.
-        assert (Z.of_nat (S n1) -1 = Z.of_nat n1) by admit.
-        rewrite H7. admit.      (* true from H9 *)
-      * simpl. unfold findChildIndex, n in FCI. rewrite FCI.
-        simpl.
-        admit.                  (* ok from Hnum *)
-  - forward_if.
-    + forward.                  (* return *)
-      rewrite H1. entailer!.
-    + forward.                  (* skip *)
-      forward.                  (* return *)
-      rewrite H1. entailer!.
-Admitted.
+Require Import verif_isnodeparent.
 
 Lemma body_AscendToParent: semax_body Vprog Gprog f_AscendToParent AscendToParent_spec.
 Proof.
