verif/verif_isnodeparent.v
@@ -1,0 +1,122 @@
+(** * verif_isnodeparent.v : Correctness proof of isNodeParent *)
+
+Require Import VST.floyd.proofauto.
+Require Import VST.floyd.library.
+Require Import relation_mem.
+Instance CompSpecs : compspecs. make_compspecs prog. Defined.
+Definition Vprog : varspecs. mk_varspecs prog. Defined.
+
+Require Import VST.msl.wand_frame.
+Require Import VST.msl.iter_sepcon.
+Require Import VST.floyd.reassoc_seq.
+Require Import VST.floyd.field_at_wand.
+Require Import FunInd.
+Require Import btrees.
+Require Import index.
+Require Import btrees_sep.
+Require Import btrees_spec.
+Require Import verif_findindex.
+
+Lemma body_isNodeParent: semax_body Vprog Gprog f_isNodeParent isNodeParent_spec.
+Proof.
+  start_function.
+  destruct n as [ptr0 le isLeaf First Last pn].
+  pose (n:=btnode val ptr0 le isLeaf First Last pn).
+  rewrite unfold_btnode_rep. Intros ent_end.
+  forward.                      (* t'5 = node->isLeaf *)
+  { entailer!. destruct isLeaf; simpl; auto. }
+  forward_if.
+{                               (* Leaf Node *)
+  assert(LEAF: isLeaf = true).
+  { destruct isLeaf; auto. simpl in H1. inv H1. } subst.
+  forward.                       (* t'10 = node->numKeys *)
+  gather_SEP 0 1 2 3. replace_SEP 0 (btnode_rep n).
+  { entailer!. rewrite unfold_btnode_rep with (n:=n). Exists ent_end. entailer!. }
+  forward_if.
+  - forward.                    (* return. *)
+    entailer!. destruct le as [|e le']. auto.
+    simpl in H2. unfold node_wf in H0. simpl in H0. rewrite Fanout_eq in H0. exfalso.
+    rewrite Zpos_P_of_succ_nat in H2. apply (f_equal Int.unsigned) in H2.
+    autorewrite with norm in H2. omega.
+  - forward.                    (* skip *)
+    assert(NELE: numKeys_le le <> O).
+    { destruct le. simpl in H2. contradiction. simpl. omega. }
+    destruct le as [|e le']. simpl in NELE. contradiction.
+    pose (le:= cons val e le'). fold le.
+    rewrite unfold_btnode_rep. clear ent_end. unfold n. Intros ent_end.
+    forward.                    (* lowest=node->entries[0]->key *)
+    { unfold le. simpl. rewrite Znth_0_cons. destruct e; simpl; entailer!. }
+    forward.                    (* t'9=node->numKeys *)
+    forward.                    (* highest=node->entries[t'9-1] *)
+    + rewrite Zpos_P_of_succ_nat. entailer!. rewrite Zsuccminusone.
+      unfold node_wf in H0. simpl in H0. rewrite Fanout_eq in H0. omega.
+    + admit.                    (* should be ok, do we need to split le? *)
+    + entailer!. rewrite Zpos_P_of_succ_nat. unfold node_wf in H0. simpl in H0. rewrite Fanout_eq in H0.
+      rewrite Int.signed_repr. rewrite Int.signed_repr.
+      rewrite Zsuccminusone. 
+      rep_omega. rep_omega. rep_omega.
+    + admit.
+} {                             (* Intern Node *)
+  assert(INTERN: isLeaf = false).
+  { destruct isLeaf; auto. simpl in H1. inv H1. } subst.
+  gather_SEP 0 1 2 3. replace_SEP 0 (btnode_rep n).
+  { entailer!. rewrite unfold_btnode_rep with (n:=n). Exists ent_end. entailer!. }
+  forward_call(n,key).
+  { split3. unfold n. simpl. auto. auto. auto. }
+  forward_if(PROP() LOCAL(temp _t'4 (Val.of_bool (negb (isNodeParent n key))); temp _idx (Vint(Int.repr((rep_index (findChildIndex n key))))); temp _node pn; temp _key (key_repr key)) SEP (btnode_rep n)).
+  - forward.                    (* t'4=1 *)
+    entailer!.
+    destruct (findChildIndex n key) eqn:FCI.
+    simpl in FCI. rewrite FCI. auto.
+    simpl in FCI. rewrite FCI in H2. simpl in H2.
+    apply (f_equal Int.unsigned) in H2.
+    assert(Z.of_nat n0 < Z.of_nat Fanout).
+    { assert(-1 <= idx_to_Z (findChildIndex n key) < Z.of_nat (numKeys n)) by apply FCI_inrange.
+      simpl in H4. rewrite FCI in H4. simpl in H4.
+      unfold node_wf in H0. simpl in H0. omega. }
+    rewrite Fanout_eq in H4. simpl in H4. autorewrite with norm in H2.
+    rewrite H2 in H4. compute in H4. inv H4.
+  - rewrite unfold_btnode_rep. unfold n. Intros ent_end0.
+    forward.                    (* t'6=node->numKeys *)
+    forward.                    (* t'4= (idx==t'6-1) *)
+    { entailer!. unfold node_wf in H0. simpl in H0. rewrite Fanout_eq in H0.
+      rewrite Int.signed_repr. rewrite Int.signed_repr.
+      rep_omega. rep_omega. rep_omega. }
+    gather_SEP 0 1 2 3. replace_SEP 0 (btnode_rep n).
+    { entailer!. rewrite unfold_btnode_rep. Exists ent_end0. entailer!. }
+    entailer!.
+    destruct (findChildIndex' le key im) eqn:FCI'.
+    { simpl in H2. contradiction. }
+    rewrite negb_involutive. simpl.
+    destruct (S n0 =? numKeys_le le)%nat eqn:HNUM.
+    + destruct (numKeys_le le).
+      apply beq_nat_true in HNUM. omega.
+      apply beq_nat_true in HNUM. inv HNUM.
+      replace (Z.of_nat (S n1) -1) with (Z.of_nat n1).
+      rewrite Int.eq_true. rewrite Nat.eqb_refl. simpl. auto.
+      rewrite Nat2Z.inj_succ. rewrite Zsuccminusone. auto.
+    + apply beq_nat_false in HNUM.
+      destruct(Int.eq (Int.repr (Z.of_nat n0)) (Int.repr (Z.of_nat (numKeys_le le) - 1))) eqn:HEQ.
+      { unfold node_wf in H0. rewrite Fanout_eq in H0. simpl in H0.
+        apply eq_sym in HEQ. apply binop_lemmas2.int_eq_true in HEQ. exfalso.
+        apply (f_equal Int.unsigned) in HEQ.
+        rewrite Int.unsigned_repr in HEQ. rewrite Int.unsigned_repr in HEQ.
+        assert(Z.of_nat (S n0) = Z.of_nat (numKeys_le le)) by omega.
+        apply Nat2Z.inj in H5. rewrite H5 in HNUM. contradiction.
+        split. destruct le. simpl in FCI'. inv FCI'. simpl numKeys_le.
+        rewrite Nat2Z.inj_succ. rewrite Zsuccminusone. omega.
+        rep_omega.
+        split. omega.
+        assert(-1 <= idx_to_Z (findChildIndex n key) < Z.of_nat (numKeys n)) by apply FCI_inrange.
+        simpl in H5. rewrite FCI' in H5. simpl in H5. rep_omega. }      
+      destruct (numKeys_le le).
+      simpl. auto. destruct (n0 =? n1)%nat eqn:HEQ2.
+      apply beq_nat_true in HEQ2. subst. contradiction. simpl. auto.      
+  - forward_if.
+    + forward.                  (* return 0 *)
+      entailer!.
+      rewrite H2. simpl. auto.
+    + forward.                  (* skip *)
+      forward.                  (* return 1 *)
+      rewrite H2. entailer!.
+Admitted.    
